dfy-compile.bat
@@ -1,14 +1,14 @@
 @echo off
 
-for %%X in (dafny.exe) do (set FOUND=%%~$PATH:X)
+for %%X in (dafny) do (set FOUND=%%~$PATH:X)
 if defined FOUND (
   if "%1" == "" goto empty
-  dafny.exe %1
+  dafny %1
   echo %~n1.dll
   goto end
 )
 :nodafny
-echo Can't find dafny.exe in %%PATH%%
+echo Can't find dafny in %%PATH%%
 echo You can get Dafny at http://dafny.codeplex.com/
 echo Press any key to open page in your browser
 pause >nul
